

# A model of type theory with quotient inductive-inductive types

Szumi Xie

Eötvös Loránd University, Budapest

j.w.w. Ambrus Kaposi

TYPES 2020

Torino, 2 March 2020



SZÉCHENYI 2020

Európai Unió  
Európai Szociális  
Alap



BEFEKTETÉS A JÖVŐBE

# Overview

- 1 Quotient inductive-inductive types (QIITs)
- 2 Specification of QIITs in a model
- 3 The setoid model
- 4 Implementation of the universal QIIT in the setoid model
- 5 Conclusion

# Plan

- 1 Quotient inductive-inductive types (QIITs)
- 2 Specification of QIITs in a model
- 3 The setoid model
- 4 Implementation of the universal QIIT in the setoid model
- 5 Conclusion

# Examples of QIITs

$\text{Con} : \text{Set}$

$\text{Ty} : \text{Con} \rightarrow \text{Set}$

$\bullet : \text{Con}$

$- \triangleright - : (\Gamma : \text{Con}) \rightarrow \text{Ty } \Gamma \rightarrow \text{Con}$

$\text{U} : \text{Ty } \Gamma$

$\text{El} : \text{Ty } (\Gamma \triangleright \text{U})$

$\Sigma : (A : \text{Ty } \Gamma) \rightarrow \text{Ty } (\Gamma \triangleright A) \rightarrow \text{Ty } \Gamma$

$\text{eq} : \Gamma \triangleright \Sigma A B = \Gamma \triangleright A \triangleright B$

Other examples: Cauchy real numbers, partiality monad, intrinsic syntax for programming languages

# What is a QIIT?

- A context in the universal QIIT.
- Universal QIIT is a syntax for a small type theory
- Example:  $\text{Nat} : \mathbf{U}$ ,  $\text{zero} : \text{El Nat}$ ,  $\text{suc} : \text{Nat} \Rightarrow \text{El Nat}$
- All QIITs can be constructed from the universal QIIT (Kaposi, Kovács, Altenkirch, POPL 2019)

# Is this definition circular?

- A model of type theory supports the universal QIIT:
  - ▶ notion of algebra
  - ▶ notion of homomorphism
  - ▶ there is an algebra (constructor)
  - ▶ for every other algebra there is a homomorphism from the constructor to that algebra (recursor)
  - ▶ the recursor is unique

# Is this definition circular?

- A model of type theory supports the universal QIIT:
  - ▶ notion of algebra
  - ▶ notion of homomorphism
  - ▶ there is an algebra (constructor)
  - ▶ for every other algebra there is a homomorphism from the constructor to that algebra (recursor)
  - ▶ the recursor is unique
- Rest of this talk:
  - ▶ How to express all of these for a model of type theory
  - ▶ Define a model which supports the universal QIIT
  - ▶ Everything was formalised in Agda

# Plan

- 1 Quotient inductive-inductive types (QIITs)
- 2 Specification of QIITs in a model
- 3 The setoid model
- 4 Implementation of the universal QIIT in the setoid model
- 5 Conclusion



# Model of type theory (i)

CwF with extra structure:

$\mathbf{Con} : \mathbf{Set}$

$\mathbf{T}_y : \mathbf{Con} \rightarrow \mathbf{Set}$

$\mathbf{Sub} : \mathbf{Con} \rightarrow \mathbf{Con} \rightarrow \mathbf{Set}$

$\mathbf{T}_m : (\Gamma : \mathbf{Con}) \rightarrow \mathbf{T}_y \Gamma \rightarrow \mathbf{Set}$

$\Pi : (A : \mathbf{T}_y \Gamma) \rightarrow \mathbf{T}_y (\Gamma \triangleright A) \rightarrow \mathbf{T}_y \Gamma$

$\mathbf{lam} : \mathbf{T}_m (\Gamma \triangleright A) B \rightarrow \mathbf{T}_m \Gamma (\Pi A B)$

$\mathbf{app} : \mathbf{T}_m \Gamma (\Pi A B) \rightarrow \mathbf{T}_m (\Gamma \triangleright A) B$

$\vdots$

# Model of type theory (ii)

$\text{Con} : \mathbb{N} \rightarrow \text{Set}$	$\Sigma : (A : \text{Ty } i \Gamma) \rightarrow \text{Ty } j (\Gamma \triangleright A) \rightarrow$
$\text{Ty} : \mathbb{N} \rightarrow \text{Con } i \rightarrow \text{Set}$	$\text{Ty } (i \sqcup j) \Gamma$
$\text{Sub} : \text{Con } i \rightarrow \text{Con } j \rightarrow \text{Set}$	$\neg, - : (u : \text{Tm } \Gamma A) \rightarrow \text{Tm } \Gamma (B[\text{id}, u]) \rightarrow$
$\text{Tm} : (\Gamma : \text{Con } i) \rightarrow \text{Ty } j \Gamma \rightarrow \text{Set}$	$\text{Tm } \Gamma (\Sigma A B)$
$\text{id} : \text{Sub } \Gamma \Gamma$	$\text{projl} : \text{Tm } \Gamma (\Sigma A B) \rightarrow \text{Tm } \Gamma A$
$- \circ - : \text{Sub } \Theta \Delta \rightarrow \text{Sub } \Gamma \Theta \rightarrow \text{Sub } \Gamma \Delta$	$\text{projr} : (t : \text{Tm } \Gamma (\Sigma A B)) \rightarrow$
$\text{ass} : (\sigma \circ \delta) \circ \nu = \sigma \circ (\delta \circ \nu)$	$\text{Tm } \Gamma (B[\text{id}, \text{projl } t])$
$\text{idl} : \text{id} \circ \sigma = \sigma$	$\Sigma \beta_1 : \text{projl } (u, v) = u$
$\text{idr} : \sigma \circ \text{id} = \sigma$	$\Sigma \beta_2 : \text{projr } (u, v) = v$
$[-] : \text{Ty } i \Delta \rightarrow \text{Sub } \Gamma \Delta \rightarrow \text{Ty } i \Gamma$	$\Sigma \eta : (\text{projl } t, \text{projr } t) = t$
$[-] : \text{Tm } \Delta A \rightarrow (\sigma : \text{Sub } \Gamma \Delta) \rightarrow$	$\Sigma [] : (\Sigma A B)[\sigma] = \Sigma (A[\sigma]) (B[\sigma^1])$
$\text{Tm } \Gamma (A[\sigma])$	$[\ ] : \langle u, v \rangle [\sigma] = \langle u[\sigma], v[\sigma] \rangle$
$[\text{id}] : A[\text{id}] = A$	$\top : \text{Ty } 0 \Gamma$
$[\sigma] : A[\sigma \circ \delta] = A[\sigma][\delta]$	$\text{tt} : \text{Tm } \Gamma \top$
$[\text{id}] : t[\text{id}] = t$	$\top \eta : (t : \text{Tm } \Gamma \top) = \text{tt}$
$[\sigma] : t[\sigma \circ \delta] = t[\sigma][\delta]$	$\top [] : \top[\sigma] = \top$
$\cdot : \text{Con } 0$	$\text{tt}[] : \text{tt}[\sigma] = \text{tt}$
$\epsilon : \text{Sub } \Gamma \cdot$	$\text{U} : (i : \mathbb{N}) \rightarrow \text{Ty } (i + 1) \Gamma$
$\cdot \eta : (\sigma : \text{Sub } \Gamma \cdot) = \epsilon$	$\text{El} : \text{Tm } \Gamma (\text{U } i) \rightarrow \text{Ty } i \Gamma$
$\triangleright - : (\Gamma : \text{Con } i) \rightarrow \text{Ty } j \Gamma \rightarrow \text{Con } (i \sqcup j)$	$\text{c} : \text{Ty } i \Gamma \rightarrow \text{Tm } \Gamma (\text{U } i)$
$\neg, - : (\sigma : \text{Sub } \Gamma \Delta) \rightarrow \text{Tm } \Gamma (A[\sigma]) \rightarrow$	$\text{U}\beta : \text{El } (\text{c } A) = A$
$\text{Sub } \Gamma (\Delta \triangleright A)$	$\text{U}\eta : \text{c } (\text{El } a) = a$
$\text{p} : \text{Sub } (\Gamma \triangleright A) \Gamma$	$\text{U}[] : \langle \text{U } i \rangle [\sigma] = \langle \text{U } i \rangle$
$\text{q} : \text{Tm } (\Gamma \triangleright A) (A[\text{p}])$	$\text{El}[] : \langle \text{El } a \rangle [\sigma] = \text{El } (a[\sigma])$
$\triangleright \beta_1 : \text{p} \circ (\sigma, t) = \sigma$	$\text{Bool} : \text{Ty } 0 \Gamma$
$\triangleright \beta_2 : \text{q}[\sigma, t] = t$	$\text{true} : \text{Tm } \Gamma \text{Bool}$
$\triangleright \eta : (\text{p}, \text{q}) = \text{id}$	$\text{false} : \text{Tm } \Gamma \text{Bool}$
$\circ : (\sigma, t) \circ \nu = (\sigma \circ \nu, t[\nu])$	$\text{if} : (C : \text{Ty } i (\Gamma \triangleright \text{Bool})) \rightarrow$
$\Pi : (A : \text{Ty } i \Gamma) \rightarrow \text{Ty } j (\Gamma \triangleright A) \rightarrow$	$\text{Tm } \Gamma (C[\text{id}, \text{true}]) \rightarrow$
$\text{Ty } (i \sqcup j) \Gamma$	$\text{Tm } \Gamma (C[\text{id}, \text{false}]) \rightarrow$
$\text{lam} : \text{Tm } (\Gamma \triangleright A) B \rightarrow \text{Tm } \Gamma (\Pi A B)$	$(t : \text{Tm } \Gamma \text{Bool}) \rightarrow \text{Tm } \Gamma (C[\text{id}, t])$
$\text{app} : \text{Tm } \Gamma (\Pi A B) \rightarrow \text{Tm } (\Gamma \triangleright A) B$	$\text{Bool}\beta_1 : \text{if } C \text{ u v true} = u$
$\Pi\beta : \text{app } (\text{lam } t) = t$	$\text{Bool}\beta_2 : \text{if } C \text{ u v false} = v$
$\Pi\eta : \text{lam } (\text{app } t) = t$	$\text{Bool}[] : \text{Bool}[\sigma] = \text{Bool}$
$\Pi[] : (\Pi A B)[\sigma] = \Pi (A[\sigma]) (B[\sigma^1])$	$\text{true}[] : \text{true}[\sigma] = \text{true}$
$\text{lam}[] : (\text{lam } t)[\sigma] = \text{lam } (t[\sigma^1])$	$\text{false}[] : \text{false}[\sigma] = \text{false}$
	$\text{if}[] : (\text{if } C \text{ u v } t)[\sigma] =$
	$\text{if } (C[\sigma^1]) (u[\sigma]) (v[\sigma]) (t[\sigma])$

# A model supports a QIIT: algebra

$\text{Con} : \text{Set}$	$\text{Con}^s : \text{Ty } \bullet$
$\text{Ty} : \text{Con} \rightarrow \text{Set}$	$\text{Ty}^s : \text{Ty } (\bullet \triangleright \text{Con}^s)$
$\text{Sub} : \text{Con} \rightarrow \text{Con} \rightarrow \text{Set}$	$\text{Sub}^s : \text{Ty } (\bullet \triangleright \text{Con}^s \triangleright \text{Con}^s[\epsilon])$
$\text{Tm} : (\Gamma : \text{Con}) \rightarrow \text{Ty } \Gamma \rightarrow \text{Set}$	$\text{Tm}^s : \text{Ty } (\bullet \triangleright \text{Con}^s \triangleright \text{Ty}^s)$
$\bullet : \text{Con}$	$\bullet^s : \text{Tm } \bullet \text{ Con}^s$
$- \triangleright - : (\Gamma : \text{Con}) \rightarrow \text{Ty } \Gamma \rightarrow \text{Con}$	$\triangleright^s : \text{Tm } (\bullet \triangleright \text{Con}^s \triangleright \text{Ty}^s) (\text{Con}^s[\epsilon])$
$\text{U} : \text{Ty } \Gamma$	$\text{U}^s : \text{Tm } (\bullet \triangleright \text{Con}^s) \text{ Ty}^s$
$\text{El} : \text{Tm } \Gamma \text{ U} \rightarrow \text{Ty } \Gamma$	$\text{El}^s : \text{Tm } (\bullet \triangleright \text{Con}^s \triangleright \text{Tm}^s[\text{id}, \text{U}^s]) (\text{Ty}^s[\text{wk}^1])$
$\Pi : (a : \text{Tm } \Gamma \text{ U}) \rightarrow$ $\text{Ty } (\Gamma \triangleright \text{El } a) \rightarrow \text{Ty } \Gamma$	$\Pi^s : \text{Tm } (\bullet \triangleright \text{Con}^s \triangleright \text{Tm}^s[\text{id}, \text{U}^s]$ $\triangleright \text{Ty}^s[\epsilon, \triangleright^s[\text{wk}^1, \text{El}^s]]) (\text{Ty}^s[\text{wk}^2])$
$\vdots$	$\vdots$

# A model supports a QIIT: implementation

$\Pi^T : \forall \text{Con}^s \text{Ty}^s \text{Tm}^s \rightarrow \blacktriangleright^T \text{Con}^s \text{Ty}^s \rightarrow \forall U^s \rightarrow \text{El}^T \text{Con}$   
 $\Pi^T \text{Con}^s \text{Ty}^s \text{Tm}^s \blacktriangleright^s U^s \text{El}^s = \text{Tm} \Pi^c \Pi^R$

module  $\Pi^T$  where

open  $\text{Con}^T$

open  $\text{Ty}^T \text{Con}^s$

open  $\text{Tm}^T \text{Con}^s \text{Ty}^s$

open  $\blacktriangleright^T \text{Con}^s \text{Ty}^s$

open  $U^T \text{Con}^s \text{Ty}^s$

open  $\text{El}^T \text{Con}^s \text{Ty}^s \text{Tm}^s U^s$

$\Pi-\Gamma = \text{Con}^s$

$\Pi-a = \text{Tm}^s [ < U^s > ]T$

$\Pi-B = \text{Ty}^s [ \varepsilon , \langle \text{Ty}-\Gamma \rangle \blacktriangleright^s [ \text{wk}^1 \Pi-a , \langle \blacktriangleright-A \rangle \text{El}$

$\Pi^c = \bullet \triangleright \Pi-\Gamma \triangleright \Pi-a \triangleright \Pi-B$

$\Pi^R = \text{Ty}^s [ \text{wk}^2 \Pi-a \Pi-B ]T$



# A model supports a QIIT: homomorphism

$$\text{Con}^M : \text{Con}_1 \rightarrow \text{Con}_2$$

$$\text{Ty}^M : \text{Ty}_1 \Gamma \rightarrow \text{Ty}_2 (\text{Con}^M \Gamma)$$

$$\text{Sub}^M : \text{Sub}_1 \Gamma \Delta \rightarrow \\ \text{Sub}_2 (\text{Con}^M \Gamma) (\text{Con}^M \Delta)$$

$$\text{Tm}^M : \text{Tm}_1 \Gamma A \rightarrow \\ \text{Tm}_2 (\text{Con}^M \Gamma) (\text{Ty}^M A)$$

$$\bullet^M : \text{Con}^M \bullet_1 = \bullet_2$$

$$\triangleright^M : \text{Con}^M (\Gamma \triangleright_1 A) = \\ (\text{Con}^M \Gamma) \triangleright_2 (\text{Ty}^M A)$$

⋮

$$\text{Con}^M : \text{Tm} (\bullet \triangleright \text{Con}_1) (\text{Con}_2 [\epsilon])$$

$$\text{Ty}^M : \text{Tm} (\bullet \triangleright \text{Con}_1 \triangleright \text{Ty}_1) (\text{Ty}_2 [\epsilon, \text{Con}^M [\text{wk}^1]])$$

$$\text{Sub}^M : \text{Tm} (\bullet \triangleright \text{Con}_1 \triangleright \text{Con}_1 [\epsilon] \triangleright \text{Sub}_1) \\ (\text{Sub}_2 [\epsilon, \text{Con}^M [\text{wk}^2], \text{Con}^M [\epsilon, v^1]])$$

$$\text{Tm}^M : \text{Tm} (\bullet \triangleright \text{Con}_1 \triangleright \text{Ty}_1 \triangleright \text{Tm}_1) \\ (\text{Tm}_2 [\epsilon, \text{Con}^M [\text{wk}^2], \text{Ty}^M [\text{wk}^1]])$$

$$\bullet^M : \text{Tm} \bullet (\text{Id} (\text{Con}^M [\epsilon, \bullet_1]) \bullet_2)$$

$$\triangleright^M : \text{Tm} (\bullet \triangleright \text{Con}_1 \triangleright \text{Ty}_1) \\ (\text{Id} (\text{Con}^M [\epsilon, \triangleright_1]) \\ (\triangleright_2 [\epsilon, \text{Con}^M [\text{wk}^1], \text{Ty}^M]))$$

⋮

# Plan

- 1 Quotient inductive-inductive types (QIITs)
- 2 Specification of QIITs in a model
- 3 The setoid model
- 4 Implementation of the universal QIIT in the setoid model
- 5 Conclusion

# The setoid model

```

record Con i : Set (lsuc i) where
  field
    |_IC : Set i
    C~ : |_IC → |_IC → Prop i
    refC : ∀ y → C~ y y
    symC : ∀{y y'} → C~ y y' → C~ y' y
    transC : ∀{y y' y''} → C~ y y' → C~ y' y'' → C~ y y''
  infix 4 |_IC
  infix 5 C~
open Con public

record Tms {i j} (Γ : Con i) (Δ : Con j) : Set (i u j) where
  field
    |_Is : | Γ |_IC → | Δ |_IC
    ~s : {y y' : | Γ |_IC} → Γ C y ~ y' → Δ C (|_Is y) ~ (|_Is y')
  infix 4 |_Is
open Tms public

record Ty {i} (Γ : Con i) j : Set (i u lsuc j) where
  constructor mkTy
  field
    |_IT_ : | Γ |_IC → Set j
    T⊢~ : ∀{y y'} (p : Γ C y ~ y') → |_IT_ y → |_IT_ y' → Prop j
    refT : ∀{y} α → T⊢~ (refC Γ y) α α
    symT : ∀{y y'} (p : Γ C y ~ y') {α : |_IT_ y} {α' : |_IT_ y'}
      → T⊢~ p α α' → T⊢~ (symC Γ p) α' α
    transT : ∀{y y' y'} (p : Γ C y ~ y') {q : Γ C y' ~ y''}
      {α : |_IT_ y} {α' : |_IT_ y'} {α'' : |_IT_ y''}
      → T⊢~ p α α' → T⊢~ q α' α'' → T⊢~ (transC Γ p q) α α''
    coeT : {y y' : | Γ |_IC} → Γ C y ~ y' → |_IT_ y → |_IT_ y'
    cohT : {y y' : | Γ |_IC} (p : Γ C y ~ y') (α : |_IT_ y) → T⊢~ p α (coeT p α)
  infix 4 |_IT_
  infix 5 T⊢~
open Ty public

record Tm {i} (Γ : Con i) {j} (A : Ty Γ j) : Set (i u j) where
  field
    |_It : (y : | Γ |_IC) → | A |_IT y
    ~t : {y y' : | Γ |_IC} (p : Γ C y ~ y') → A T p ⊢ (|_It y) ~ (|_It y')
  infix 4 |_It
open Tm public

```



# Plan

- 1 Quotient inductive-inductive types (QIITs)
- 2 Specification of QIITs in a model
- 3 The setoid model
- 4 Implementation of the universal QIIT in the setoid model**
- 5 Conclusion

# Implementation IIT (i)

```
data Con   : Set1
data Ty    : Con → Set1
data Sub   : Con → Con → Set1
data Tm    : (Γ : Con) → Ty Γ → Set1
```

```
data Con~   : Con → Con → Prop1
data Ty~    : ∀ {Γ0 Γ1} → Con~ Γ0 Γ1 → Ty Γ0 → Ty Γ1 → Prop1
data Sub~   : ∀ {Γ0 Γ1} → Con~ Γ0 Γ1 → ∀ {Δ0 Δ1} → Con~ Δ0 Δ1 → Sub Γ0 Δ0 → Sub Γ1 Δ1
data Tm~    : ∀ {Γ0 Γ1} (Γ01 : Con~ Γ0 Γ1) {A0 A1} → Ty~ Γ01 A0 A1 → Tm Γ01 A0 A1
```

⋮

```
data Ty where
```

```
U      : ∀ {Γ} → Ty Γ
El     : ∀ {Γ} → Tm Γ U → Ty Γ
Π      : ∀ {Γ} (a : Tm Γ U) → Ty (Γ ▶ El a) → Ty Γ
Id     : ∀ {Γ} (a : Tm Γ U) (u v : Tm Γ (El a)) → Ty Γ
_[]_T  : ∀ {Γ Δ} → Ty Δ → Sub Γ Δ → Ty Γ
coerce : ∀ {Γ0 Γ1} → Con~ Γ0 Γ1 → Ty Γ0 → Ty Γ1
```

⋮

# Implementation IIT (ii)

data Ty~ where

rfiT :  $\forall \{\Gamma \ A\} \rightarrow \text{Ty~} \{\Gamma\}\{\Gamma\} \text{ rfiC } A \ A$

symT :  $\forall \{\Gamma_0 \ \Gamma_1 \ \Gamma_{01} \ A_0 \ A_1\} \rightarrow \text{Ty~} \{\Gamma_0\}\{\Gamma_1\} \ \Gamma_{01} \ A_0 \ A_1 \rightarrow$

trst :  $\forall \{\Gamma_0 \ \Gamma_1 \ \Gamma_2 \ \Gamma_{01} \ \Gamma_{12}\}\{A_0 \ A_1 \ A_2\} \rightarrow \text{Ty~} \{\Gamma_0\}\{\Gamma_1\} \ \Gamma_{01} \ A_0 \ A_1 \rightarrow$   
 $\rightarrow \text{Ty~} (\text{trstC } \Gamma_{01} \ \Gamma_{12}) \ A_0 \ A_2$

cohT :  $\forall \{\Gamma_0 \ \Gamma_1\}(\Gamma_{01} : \text{Con~} \Gamma_0 \ \Gamma_1)(A : \text{Ty } \Gamma_0) \rightarrow \text{Ty~} \Gamma_{01} \ A \ A$

U~ :  $\forall \{\Gamma_0 \ \Gamma_1 \ \Gamma_{01}\} \rightarrow \text{Ty~} \{\Gamma_0\}\{\Gamma_1\} \ \Gamma_{01} \ U \ U$

El~ :  $\forall \{\Gamma_0 \ \Gamma_1 \ \Gamma_{01}\}\{t_0 : \text{Tm } \Gamma_0 \ U\}\{t_1 : \text{Tm } \Gamma_1 \ U\} \rightarrow \text{Tm~} \Gamma_{01} \ t_0 \ t_1$

⋮

U[] :  $\forall \{\Gamma \ \Delta\}\{\sigma : \text{Sub } \Gamma \ \Delta\} \rightarrow \text{Ty~} \text{rfiC } (U \ [ \ \sigma \ ]T) \ U$

El[] :  $\forall \{\Gamma \ \Delta\}\{\sigma : \text{Sub } \Gamma \ \Delta\}\{a : \text{Tm } \Delta \ U\} \rightarrow \text{Ty~} \text{rfiC } (\text{El } a \ [ \ \sigma \ ]T) \ (\text{El } (\text{coerce rfiC } U[]) \ a)$

⋮

# Constructors

```

Tys : TyT Cons
| Tys |T _ ,Σ Γs = S.Ty Γs
T ⊢ ~ Tys ( _ ,p Γs~ ) = S.Ty~ Γs~
refT Tys _ = S.rflT
symT Tys _ = S.symT
transT Tys = S.trsT
coeT Tys ( _ ,p Γs ) = S.coerce Γs
cohT Tys ( _ ,p Γs ) = S.cohT Γs

```

```

Us : UT Cons Tys
| Us |t _ = S.U
~t Us _ = S.U~

```

```

Els : ElT Cons Tys Tms Us
| Els |t ( _ ,Σ As ) = S.El As
~t Els ( _ ,p As~ ) = S.El~ As~

```

```

U[]s : U[]T Cons Tys Subs []Ts Us
| U[]s |t _ = liftp S.U[]
~t U[]s = _

```

```

El[]s : El[]T Cons Tys Subs Tms []Ts []s Us Els U[]s
| El[]s |t _ = liftp S.El[]
~t El[]s = _

```

# Recursor

```

recIx : S.Ix → Prop
recCon : S.Con → Cons
recTy : ∀{Γ} → S.Ty Γ → Tys
recSub : ∀{Γ Δ} → S.Sub Γ Δ → Subs
recTm : ∀{Γ A} → S.Tm Γ A → Tms
recCll : {i : S.Ix} → S.Cll i → recIx i

recIx (S.Con-I Γ0 Γ1) = Cons T _ ⊢ recCon Γ0 ~ recCon Γ1
recIx (S.Ty-I Γ0 A0 A1) = Tys T _ ,p recCll Γ0 ⊢ recTy A0 ~ recTy A1
recIx (S.Sub-I Γ0 Δ0 Δ1 Δ0 Δ1) = Subs T _ ,p recCll Γ0 ,p recCll Δ0 ⊢ recSub Δ0 ~ recSub Δ1
recIx (S.Tm-I Γ0 A0 t0 t1) = Tms T _ ,p recCll Γ0 ,p recCll A0 ⊢ recTm t0 ~ recTm t1

recCon S.★ = | ★s T _
recCon (S.► A) = | ►s T _ ,Σ recTy A

recTy S.U = | Us T _
recTy (S.El a) = | Els T _ ,Σ recTm a
recTy (S.coerce Γ0 A) = coeT Tys ( _ ,p recCll Γ0) (recTy A)

:

recCll S.★ = ~t ★s
recCll (S.► _ A01) = ~t ►s T _ ,p recCll A01
recCll S.rflC = refl Cons
recCll (S.symC Γ01) = symT Cons T (recCll Γ01)
recCll (S.trnC Γ01 Γ12) = transT Cons (recCll Γ01) (recCll Γ12)

recCll S.U = ~t Us
recCll (S.El ~ Γ01 = Γ01) a01 = ~t Els T _ ,p recCll Γ01 ,p recCll a01
recCll (S.cohT _ ) = cohT Tys _
recCll S.rflT = refl Tys
recCll (S.symT A01) = symT Tys T (recCll A01)
recCll (S.trnT A01 A12) = transT Tys T (recCll A01) (recCll A12)
recCll S.U[] = | U[]s T _ .unliftp
recCll S.El[] = | El[]s T _ .unliftp

:

recCons : ConHT S.Cons Cons
| recCons T ( _ ,Σ Γ ) = recCon Γ
~t recCons ( _ ,p Γ01) = recCll Γ01

recTys : TyHT S.Cons Cons recCons S.Tys Tys
| recTys T ( _ ,Σ A ) = recTy A
~t recTys ( _ ,p A01) = recCll A01

:

```

# Uniqueness

```

uniqCon : ∀ Γ → Cons T- ⊢ | Conm | t ( _ , Σ Γ ) ~ recCon Γ
uniqTy   : ∀{Γ} A → Tys T- ,p uniqCon Γ ⊢ | Tym | t ( _ , Σ A ) ~ recTy A
uniqSub  : ∀{Γ Δ} σ → Subs T- ,p uniqCon Γ ,p uniqCon Δ ⊢ | Subm | t ( _ , Σ σ ) ~ recSub σ
uniqTm   : ∀{Γ A} t → Tms T- ,p uniqCon Γ ,p uniqTy A ⊢ | Tmm | t ( _ , Σ t ) ~ recTm t

uniqCon S.⋆ = | ⋆m | t _ .unliftp
uniqCon (Γ S.► A)
  = transT Cons ( | ►m | t _ .unliftp ) (~t ►s ( _ ,p uniqCon Γ ,p uniqTy A ))

uniqTy S.U = transT Tys ( | Um | t _ .unliftp ) (~t Us ( _ ,p uniqCon _ ))
uniqTy (S.El a)
  = transT Tys ( | Elm | t _ .unliftp )
    (~t Els ( _ ,p uniqCon _ ,p transT Tms (symT Tms (cohT Tms _ _)) (uniqTm a)))
uniqTy (S.Π a B)
  = transT Tys ( | Πm | t _ .unliftp )
    (~t Πs ( _ ,p uniqCon _ ,p transT Tms (symT Tms (cohT Tms _ _)) (uniqTm a)
      ,p transT Tys (symT Tys (cohT Tys _ _))
      (transT Tys (symT Tys (cohT Tys _ _)) (uniqTy B))))
uniqTy (S.Id a u v)
  = transT Tys ( | Idm | t _ .unliftp )
    (~t Ids ( _ ,p uniqCon _ ,p transT Tms (symT Tms (cohT Tms _ _)) (uniqTm a)
      ,p transT Tms (symT Tms (cohT Tms _ _)) (uniqTm u)
      ,p transT Tms (symT Tms (cohT Tms _ _)) (uniqTm v)))
uniqTy (A S.[ σ ]T)
  = transT Tys ( | [ ]Tm | t _ .unliftp )
    (~t [ ]Ts ( _ ,p uniqCon _ ,p uniqCon _ ,p uniqTy A ,p uniqSub σ ))
uniqTy (S.coerce Γ01 A)
  = transT Tys (~t Tym ( _ ,p S.symC Γ01 ,p S.symT (S.cohT _ _)))
    (transT Tys (uniqTy A) (cohT Tys _ _))
:

```

# Plan

- 1 Quotient inductive-inductive types (QIITs)
- 2 Specification of QIITs in a model
- 3 The setoid model
- 4 Implementation of the universal QIIT in the setoid model
- 5 Conclusion

# Conclusion

- A QIIT is a context in the universal QIIT
- All QIITs can be reduced to the universal QIIT
- We showed that the setoid model of type theory supports the universal QIIT
- All of this formalised in Agda, links in the pdf abstract



# Further work

- Infinitary QIITs
- Equalities of sorts
- Reduction rules of arbitrary QIITs constructed from the universal QIIT

